-

coq/Series.v
@@ -1,141 +1,49 @@
-(* $Id: Series.v,v 1.26 2013-07-27 00:43:35 deraugla Exp $ *)
+(* $Id: Series.v,v 1.27 2013-07-27 08:24:49 deraugla Exp $ *)
 
 Require Import Utf8.
 Require Import QArith.
+Require Import NPeano.
 
 Require Import Field.
 
 Set Implicit Arguments.
 
-CoInductive series α :=
-  | Term : α → series α → series α
-  | End : series α.
+Record series α :=
+  { terms : nat → α;
+    stop : option nat }.
 
-Definition series_hd α (s : series α) :=
-  match s with
-  | Term a _ => Some a
-  | End => None
-  end.
-
-Definition series_tl α (s : series α) : option (series α) :=
-  match s with
-  | Term _ t => Some t
-  | End => None
-  end.
-
-Fixpoint series_nth_tl α (n : nat) (s : series α) : option (series α) :=
-  match n with
-  | O => Some s
-  | S m =>
-      match series_tl s with
-      | None => None
-      | Some t => series_nth_tl m t
-      end
-  end.
-
-Definition series_nth α (n : nat) (s : series α) : option α :=
-  match series_nth_tl n s with
-  | None => None
-  | Some t => series_hd t
-  end.
-
-CoFixpoint series_map α β (f : α → β) s :=
-  match s with
-  | Term a t => Term (f a) (series_map f t)
-  | End => End _
-  end.
-
-CoInductive series_forall α P (s : series α) : Prop :=
-  | TermAndFurther : ∀ a t,
-      s = Term a t → P a → series_forall P t → series_forall P s
-  | EndOk :
-      s = End _ → series_forall P s.
-
-CoInductive eq_series α fld : series α → series α → Prop :=
-  | eq_ser_term : ∀ t₁ t₂ s₁ s₂,
-      fld_eq fld t₁ t₂
-      → eq_series fld s₁ s₂
-        → eq_series fld (Term t₁ s₁) (Term t₂ s₂)
-  | eq_ser_end :
-      eq_series fld (End _) (End _).
-
-Lemma eq_series_inv_term : ∀ α (fld : field α) t₁ t₂ s₁ s₂,
-  eq_series fld (Term t₁ s₁) (Term t₂ s₂)
-  → fld_eq fld t₁ t₂ ∧ eq_series fld s₁ s₂.
-Proof.
-intros α fld t₁ t₂ s₁ s₂ H.
-inversion H; split; assumption.
-Qed.
-
-Lemma eq_series_inv_term_end : ∀ α (fld : field α) t s,
-  ¬ eq_series fld (Term t s) (End _).
-Proof.
-intros α fld t s H.
-inversion H; contradiction.
-Qed.
-
-Lemma eq_series_inv_end_term : ∀ α (fld : field α) t s,
-  ¬ eq_series fld (End _) (Term t s).
-Proof.
-intros α fld t s H.
-inversion H; contradiction.
-Qed.
-
-Lemma eq_series_inv : ∀ α (fld : field α) s₁ s₂,
-  eq_series fld s₁ s₂
-  → (∃ t₁ t₂ s₃ s₄,
-     s₁ = Term t₁ s₃ ∧ s₂ = Term t₂ s₄ ∧
-     fld_eq fld t₁ t₂ ∧ eq_series fld s₃ s₄)
-    ∨ (s₁ = End _ ∧ s₂ = End _).
-Proof.
-intros α fld s₁ s₂ H.
-inversion H; [ left | right ].
- exists t₁, t₂, s₁0, s₂0.
- split; [ reflexivity | idtac ].
- split; [ reflexivity | idtac ].
- split; assumption.
-
- split; reflexivity.
-Qed.
+Inductive eq_series α fld : series α → series α → Prop :=
+  eq_ser' : ∀ s₁ s₂,
+    (∀ i, fld_eq fld (terms s₁ i) (terms s₂ i))
+    → stop s₁ = stop s₂
+      → eq_series fld s₁ s₂.
 
 Theorem eq_series_refl : ∀ α (fld : field α), reflexive _ (eq_series fld).
 Proof.
-cofix IHs.
 intros α fld s.
-destruct s as [t s₂| ].
- eapply eq_ser_term; try reflexivity; [ apply fld_eq_refl | apply IHs ].
-
- apply eq_ser_end; reflexivity.
+constructor; [ idtac | reflexivity ].
+intros; apply fld_eq_refl.
 Qed.
 
 Theorem eq_series_sym : ∀ α (fld : field α), symmetric _ (eq_series fld).
 Proof.
-cofix IHs.
 intros α fld s₁ s₂ H.
-destruct s₁ as [t₁ s₁| ], s₂ as [t₂ s₂| ].
- eapply eq_ser_term; try reflexivity.
-  apply eq_series_inv_term in H; destruct H.
-  apply fld_eq_sym; assumption.
-
-  apply eq_series_inv_term in H; destruct H.
-  apply IHs; assumption.
-
- apply eq_series_inv_term_end in H; contradiction.
-
- apply eq_series_inv_end_term in H; contradiction.
-
- assumption.
+inversion H; subst.
+constructor; [ idtac | symmetry; assumption ].
+intros i.
+apply fld_eq_sym.
+apply H0.
 Qed.
 
 Theorem eq_series_trans : ∀ α (fld : field α), transitive _ (eq_series fld).
 Proof.
-cofix IHs.
 intros α fld s₁ s₂ s₃ H₁ H₂.
-inversion H₁; subst; [ idtac | assumption ].
-inversion H₂; subst; constructor.
- eapply fld_eq_trans; eassumption.
+inversion H₁; inversion H₂; subst.
+constructor.
+ intros.
+ eapply fld_eq_trans; [ apply H | apply H3 ].
 
- eapply IHs; eassumption.
+ transitivity (stop s₂); assumption.
 Qed.
 
 Add Parametric Relation α (fld : field α) : (series α) (eq_series fld)
@@ -144,61 +52,28 @@ Add Parametric Relation α (fld : field α) : (series α) (eq_series fld)
  transitivity proved by (eq_series_trans (fld := fld))
  as eq_series_rel.
 
-Lemma series_eta : ∀ α (s : series α),
-  s = (match s with Term t₁ s₁ => Term t₁ s₁ | End => End _ end).
-Proof.
-intros α s.
-destruct s; reflexivity.
-Qed.
-
-Lemma series_forall_inv : ∀ α (P : α → Prop) t s,
-  series_forall P (Term t s)
-  → P t ∧ series_forall P s.
-Proof.
-intros α P t s H.
-inversion H; [ idtac | discriminate H0 ].
-injection H0; intros; subst s t; split; assumption.
-Qed.
-
-Lemma series_forall_map : ∀ α (P Q : _ → Prop) (s : series α),
-  (∀ x, P x → Q x) → series_forall P s → series_forall Q s.
-Proof.
-cofix IHs.
-intros α P Q s Hx H.
-destruct s as [t₁ s₁| ].
- apply series_forall_inv in H.
- destruct H as (H₁, H₂).
- eapply TermAndFurther; [ reflexivity | apply Hx, H₁ | idtac ].
- eapply IHs; eassumption.
-
- constructor; reflexivity.
-Qed.
-
-CoFixpoint series_add α (fld : field α) s₁ s₂ :=
-  match s₁ with
-  | Term c₁ ss₁ =>
-      match s₂ with
-      | Term c₂ ss₂ => Term (add fld c₁ c₂) (series_add fld ss₁ ss₂)
-      | End => s₁
-      end
-  | End => s₂
-  end.
+Definition series_add α (fld : field α) s₁ s₂ :=
+  {| terms := λ i, add fld (terms s₁ i) (terms s₂ i);
+     stop :=
+       match stop s₁ with
+       | Some st₁ =>
+           match stop s₂ with
+           | Some st₂ => Some (max st₁ st₂)
+           | None => None
+           end
+       | None => None
+       end |}.
 
 Lemma series_add_comm : ∀ α (fld : field α) s₁ s₂,
   eq_series fld (series_add fld s₁ s₂) (series_add fld s₂ s₁).
 Proof.
-cofix IHs; intros.
-rewrite series_eta.
-remember (series_add fld s₁ s₂) as x.
-rewrite series_eta in Heqx; subst x.
-simpl.
-destruct s₁ as [t₁ s₃| ].
- destruct s₂ as [t₂ s₄| ].
-  constructor; try reflexivity; [ apply fld_add_comm | apply IHs ].
+intros α fld s₁ s₂.
+constructor; simpl.
+ intros i.
+ apply fld_add_comm.
 
-  constructor; try reflexivity; apply fld_eq_refl.
-
- destruct s₂; reflexivity.
+ destruct (stop s₁), (stop s₂); try reflexivity.
+ rewrite Nat.max_comm; reflexivity.
 Qed.
 
 Lemma series_add_assoc : ∀ α (fld : field α) s₁ s₂ s₃,
@@ -206,14 +81,17 @@ Lemma series_add_assoc : ∀ α (fld : field α) s₁ s₂ s₃,
     (series_add fld (series_add fld s₁ s₂) s₃)
     (series_add fld s₁ (series_add fld s₂ s₃)).
 Proof.
-cofix IHs; intros.
-rewrite series_eta; symmetry.
-rewrite series_eta; symmetry.
+intros α fld s₁ s₂ s₃.
+unfold series_add.
 simpl.
-destruct s₁ as [t₁ s₁| ].
- destruct s₂ as [t₂ s₂| ].
-  destruct s₃ as [t₃ s₃| ].
-   constructor; [ apply fld_add_assoc | idtac ].
-   clear t₁ t₂ t₃.
-   Focus 1.
-bbb.
+constructor; simpl.
+ intros i.
+ apply fld_add_assoc.
+
+ destruct (stop s₁) as [a| ]; [ idtac | reflexivity ].
+ destruct (stop s₂) as [b| ]; [ idtac | reflexivity ].
+ destruct (stop s₃) as [c| ]; [ idtac | reflexivity ].
+ f_equal.
+ symmetry.
+ apply Nat.max_assoc.
+Qed.
